src/SepExpr.v
@@ -28,7 +28,6 @@ Module Type SepExprType.
 
     Definition predicates : Type := list ssignature.
 
-
     Parameter Default_predicate : ssignature.
 
     Inductive sexpr : Type :=
@@ -44,24 +43,24 @@ Module Type SepExprType.
       Variable funcs : functions types.
       Variable preds : predicates.
       
-      Fixpoint sexprD (uvs vs : env types) (s : sexpr)
+      Fixpoint sexprD (meta_env var_env : env types) (s : sexpr)
         : ST.hprop (tvarD types pcType) (tvarD types stateType) nil :=
         match s with 
           | Emp => ST.emp _ _
           | Inj p =>
-            match exprD funcs uvs vs p tvProp with
+            match exprD funcs meta_env var_env p tvProp with
               | None => ST.inj (PropX.Inj False)
               | Some p => ST.inj (PropX.Inj p)
             end
           | Star l r =>
-            ST.star (sexprD uvs vs l) (sexprD uvs vs r)
+            ST.star (sexprD meta_env var_env l) (sexprD meta_env var_env r)
           | Exists t b =>
-            ST.ex (fun x : tvarD types t => sexprD uvs (@existT _ _ t x :: vs) b)
+            ST.ex (fun x : tvarD types t => sexprD meta_env (@existT _ _ t x :: var_env) b)
           | Func f b =>
             match nth_error preds f with
               | None => ST.inj (PropX.Inj False)
               | Some f =>
-                match applyD (@exprD types funcs uvs vs) (SDomain f) b _ (SDenotation f) with
+                match applyD (@exprD types funcs meta_env var_env) (SDomain f) b _ (SDenotation f) with
                   | None => ST.inj (PropX.Inj False)
                   | Some p => p
                 end
@@ -69,15 +68,15 @@ Module Type SepExprType.
           | Const p => p
         end.
 
-    Definition himp (U1 U2 G : env types)
+    Definition himp (meta_env var_env : env types)
       (cs : codeSpec (tvarD types pcType) (tvarD types stateType))
       (gl gr : sexpr) : Prop :=
-      ST.himp cs (sexprD U1 G gl) (sexprD U2 G gr).
+      ST.himp cs (sexprD meta_env var_env gl) (sexprD meta_env var_env gr).
 
-    Definition heq (U1 U2 G : env types)
+    Definition heq (meta_env var_env : env types)
       (cs : codeSpec (tvarD types pcType) (tvarD types stateType))
       (gl gr : sexpr) : Prop :=
-      ST.heq cs (sexprD U1 G gl) (sexprD U2 G gr).
+      ST.heq cs (sexprD meta_env var_env gl) (sexprD meta_env var_env gr).
 
     End funcs_preds.
 
@@ -93,6 +92,12 @@ Module Type SepExprType.
 
     Parameter hash : sexpr -> variables * SHeap.
 
+
+    (** TODO: What happens if I denote this directly to hprop?
+     ** - fewer lemmas about concrete syntax!
+     ** - can't re-hash (probably don't want to do this anyways...)
+     ** * I think this is Ok for now
+     **)
     Parameter sheapD : SHeap -> sexpr.
 
 (*
@@ -143,24 +148,24 @@ Module Make (ST' : SepTheoryX.SepTheoryXType) <: SepExprType with Module ST := S
     | Const : ST.hprop (tvarD types pcType) (tvarD types stateType) nil -> sexpr
     .
 
-    Fixpoint sexprD (uvs vs : env types) (s : sexpr)
+    Fixpoint sexprD (meta_env var_env : env types) (s : sexpr)
       : ST.hprop (tvarD types pcType) (tvarD types stateType) nil :=
       match s with 
         | Emp => ST.emp _ _
         | Inj p =>
-          match exprD funcs uvs vs p tvProp with
+          match exprD funcs meta_env var_env p tvProp with
             | None => ST.inj (PropX.Inj False)
             | Some p => ST.inj (PropX.Inj p)
           end
         | Star l r =>
-          ST.star (sexprD uvs vs l) (sexprD uvs vs r)
+          ST.star (sexprD meta_env var_env l) (sexprD meta_env var_env r)
         | Exists t b =>
-          ST.ex (fun x : tvarD types t => sexprD uvs (@existT _ _ t x :: vs) b)
+          ST.ex (fun x : tvarD types t => sexprD meta_env (@existT _ _ t x :: var_env) b)
         | Func f b =>
           match nth_error sfuncs f with
             | None => ST.inj (PropX.Inj False)
             | Some f =>
-              match applyD (@exprD types funcs uvs vs) (SDomain f) b _ (SDenotation f) with
+              match applyD (@exprD types funcs meta_env var_env) (SDomain f) b _ (SDenotation f) with
                 | None => ST.inj (PropX.Inj False)
                 | Some p => p
               end
@@ -168,122 +173,122 @@ Module Make (ST' : SepTheoryX.SepTheoryXType) <: SepExprType with Module ST := S
         | Const p => p
       end.
 
-    Definition himp (U1 U2 G : env types)
+    Definition himp (meta_env var_env : env types)
       (cs : codeSpec (tvarD types pcType) (tvarD types stateType))
       (gl gr : sexpr) : Prop :=
-      ST.himp cs (sexprD U1 G gl) (sexprD U2 G gr).
+      ST.himp cs (sexprD meta_env var_env gl) (sexprD meta_env var_env gr).
 
-    Definition heq (U1 U2 G : env types)
+    Definition heq (meta_env var_env : env types)
       (cs : codeSpec (tvarD types pcType) (tvarD types stateType))
       (gl gr : sexpr) : Prop :=
-      ST.heq cs (sexprD U1 G gl) (sexprD U2 G gr).
+      ST.heq cs (sexprD meta_env var_env gl) (sexprD meta_env var_env gr).
 
     Section Facts.
       Variables U G : env types.
       Variable cs : codeSpec (tvarD types pcType) (tvarD types stateType).
 
-      Global Instance Trans_himp : Transitive (@himp U U G cs).
+      Global Instance Trans_himp : Transitive (@himp U G cs).
       Proof.
         red. unfold himp. intros; etransitivity; eauto.
       Qed.
 
-      Global Instance Trans_heq : Transitive (@heq U U G cs).
+      Global Instance Trans_heq : Transitive (@heq U G cs).
       Proof.
         red. unfold heq. intros; etransitivity; eauto.
       Qed.
 
-      Global Instance Refl_himp : Reflexive (@himp U U G cs).
+      Global Instance Refl_himp : Reflexive (@himp U G cs).
       Proof.
         red; unfold himp; intros. reflexivity.
       Qed.
 
-      Global Instance Refl_heq : Reflexive (@heq U U G cs).
+      Global Instance Refl_heq : Reflexive (@heq U G cs).
       Proof.
         red; unfold heq; intros. reflexivity.
       Qed.
 
-      Global Instance Sym_heq : Symmetric (@heq U U G cs).
+      Global Instance Sym_heq : Symmetric (@heq U G cs).
       Proof.
         red; unfold heq; intros. symmetry. auto.    
       Qed.
 
-      Add Parametric Relation : sexpr (@himp U U G cs)
+      Add Parametric Relation : sexpr (@himp U G cs)
         reflexivity proved by  Refl_himp
         transitivity proved by Trans_himp
       as himp_rel.
 
-      Add Parametric Relation : sexpr (@heq U U G cs)
+      Add Parametric Relation : sexpr (@heq U G cs)
         reflexivity proved by  Refl_heq
         symmetry proved by Sym_heq
         transitivity proved by Trans_heq
       as heq_rel.
 
-      Global Add Parametric Morphism U' : Star with
-        signature (himp U U' G cs ==> himp U U' G cs ==> himp U U' G cs)      
+      Global Add Parametric Morphism : Star with
+        signature (himp U G cs ==> himp U G cs ==> himp U G cs)      
         as star_himp_mor.
         unfold himp; simpl; intros; eapply SEP_FACTS.star_himp_mor; eauto.
       Qed.
 
-      Global Add Parametric Morphism U' : Star with
-        signature (heq U U' G cs ==> heq U U' G cs ==> heq U U' G cs)      
+      Global Add Parametric Morphism : Star with
+        signature (heq U G cs ==> heq U G cs ==> heq U G cs)      
         as star_heq_mor.
         unfold himp; simpl; intros; eapply SEP_FACTS.star_heq_mor; eauto.
       Qed.
 
-      Global Add Parametric Morphism U' : (himp U U' G cs) with 
-        signature (heq U U G cs ==> heq U' U' G cs ==> Basics.impl)
+      Global Add Parametric Morphism : (himp U G cs) with 
+        signature (heq U G cs ==> heq U G cs ==> Basics.impl)
         as himp_heq_mor.
         unfold heq; simpl; intros. eapply SEP_FACTS.himp_heq_mor; eauto.
       Qed.
 
-      Global Add Parametric Morphism U' : (himp U U' G cs) with 
-        signature (himp U U G cs --> himp U' U' G cs ++> Basics.impl)
+      Global Add Parametric Morphism : (himp U G cs) with 
+        signature (himp U G cs --> himp U G cs ++> Basics.impl)
         as himp_himp_mor.
         unfold himp; simpl; intros. eapply SEP_FACTS.himp_himp_mor; eauto.
       Qed.
 
       Global Add Parametric Morphism : (sexprD U G) with 
-        signature (heq U U G cs ==> ST.heq cs)
+        signature (heq U G cs ==> ST.heq cs)
         as heq_ST_heq_mor.
         unfold heq; simpl; auto.
       Qed.
 
       Lemma heq_star_emp_r : forall P, 
-        heq U U G cs (Star P Emp) P.
+        heq U G cs (Star P Emp) P.
       Proof.
         unfold heq; simpl; intros; autorewrite with hprop; reflexivity.
       Qed.
 
       Lemma heq_star_emp_l : forall P, 
-        heq U U G cs (Star Emp P) P.
+        heq U G cs (Star Emp P) P.
       Proof.
         unfold heq; simpl; intros; autorewrite with hprop; reflexivity.
       Qed.
 
       Lemma heq_star_assoc : forall P Q R, 
-        heq U U G cs (Star (Star P Q) R) (Star P (Star Q R)).
+        heq U G cs (Star (Star P Q) R) (Star P (Star Q R)).
       Proof.
         unfold heq; simpl; intros; autorewrite with hprop. rewrite ST.heq_star_assoc. reflexivity.
       Qed.
 
       Lemma heq_star_comm : forall P Q, 
-        heq U U G cs (Star P Q) (Star Q P).
+        heq U G cs (Star P Q) (Star Q P).
       Proof.
         unfold heq; simpl; intros; apply ST.heq_star_comm.
       Qed.
 
       Lemma heq_star_frame : forall P Q R S, 
-        heq U U G cs P R ->
-        heq U U G cs Q S ->
-        heq U U G cs (Star P Q) (Star R S).
+        heq U G cs P R ->
+        heq U G cs Q S ->
+        heq U G cs (Star P Q) (Star R S).
       Proof.
         unfold heq; simpl; intros. eapply ST.heq_star_frame; auto.
       Qed.
       
-      Lemma himp_star_frame : forall a b c cs P Q R S,
-        himp a b c cs P R ->
-        himp a b c cs Q S ->
-        himp a b c cs (Star P Q) (Star R S).
+      Lemma himp_star_frame : forall a c cs P Q R S,
+        himp a c cs P R ->
+        himp a c cs Q S ->
+        himp a c cs (Star P Q) (Star R S).
       Proof.
         unfold himp; simpl; intros. rewrite H; rewrite H0; reflexivity.
       Qed.
@@ -294,16 +299,16 @@ Module Make (ST' : SepTheoryX.SepTheoryXType) <: SepExprType with Module ST := S
     Existing Instance heq_rel_relation.
     Hint Rewrite heq_star_emp_l heq_star_emp_r : hprop.
 
-    Theorem ST_himp_himp : forall (U1 U2 G : env types) cs L R,
-      himp U1 U2 G cs L R ->
-      ST.himp cs (sexprD U1 G L) (sexprD U2 G R).
+    Theorem ST_himp_himp : forall (U G : env types) cs L R,
+      himp U G cs L R ->
+      ST.himp cs (sexprD U G L) (sexprD U G R).
     Proof.
       clear. auto.
     Qed.
 
-    Theorem ST_heq_heq : forall (U1 U2 G : env types) cs L R,
-      heq U1 U2 G cs L R ->
-      ST.heq cs (sexprD U1 G L) (sexprD U2 G R).
+    Theorem ST_heq_heq : forall (U G : env types) cs L R,
+      heq U G cs L R ->
+      ST.heq cs (sexprD U G L) (sexprD U G R).
     Proof.
       clear. auto.
     Qed.
@@ -323,6 +328,9 @@ Module Make (ST' : SepTheoryX.SepTheoryXType) <: SepExprType with Module ST := S
        ; other   := nil
        |}.
 
+    (** lift all the "real" variables in [a,...) 
+     ** to the range [a+b,...)
+     **)
     Fixpoint liftSExpr (a b : nat) (s : sexpr) : sexpr :=
       match s with
         | Emp => Emp
@@ -334,21 +342,18 @@ Module Make (ST' : SepTheoryX.SepTheoryXType) <: SepExprType with Module ST := S
         | Const c => Const c
       end.
 
-    (** lift all the "real" variables in [a,...) 
-     ** to the range [a+b,...)
-     **)
     Definition liftSHeap (a b : nat) (s : SHeap) : SHeap :=
       {| impures := FM.map (fun _ => map (map (liftExpr a b))) (impures s)
        ; pures   := map (liftExpr a b) (pures s)
        ; other   := other s
        |}.
 
-    Fixpoint multimap_join T (l r : FM.t (list T)) : FM.t (list T) :=
-      FM.fold (fun k v a =>
+    Definition multimap_join := 
+      FM.fold (fun (k : nat) (v : list (list (expr types))) a =>
         match FM.find k a with
           | None => FM.add k v a
           | Some v' => FM.add k (v ++ v') a
-        end) l r.
+        end).
 
     Fixpoint star_SHeap (l r : SHeap) : SHeap :=
       {| impures := multimap_join (impures l) (impures r)
@@ -356,40 +361,32 @@ Module Make (ST' : SepTheoryX.SepTheoryXType) <: SepExprType with Module ST := S
        ; other := other l ++ other r
        |}.
 
-    Fixpoint substV types (vs : list nat) (e : expr types) : expr types :=
-      match e with
-        | Expr.Const _ c => Expr.Const c
-        | Var x => 
-          Var (match nth_error vs x with
-                 | None => x
-                 | Some y => y
-               end)
-        | UVar x => UVar x
-        | Expr.Func f xs => 
-          Expr.Func f (map (substV vs) xs)
-        | Equal t e1 e2 => Equal t (substV vs e1) (substV vs e2)
-      end.
+    Definition sheap_liftVars (from : nat) (delta : nat) (h : SHeap) : SHeap :=
+      {| impures := FM.map (fun _ => map (map (liftExpr from delta))) (impures h)
+       ; pures := map (liftExpr from delta) (pures h)
+       ; other := other h
+       |}.
 
-    (** convert the sexpr into a SHeap **)
-    Fixpoint hash' (nextVar : nat) (vs : list nat) (s : sexpr) : ( variables * SHeap ) :=
+    Fixpoint hash (s : sexpr) : ( variables * SHeap ) :=
       match s with
         | Emp => (nil, SHeap_empty)
         | Inj p => (nil,
           {| impures := FM.empty
-            ; pures := p :: nil
-            ; other := nil
-          |})
+           ; pures := p :: nil
+           ; other := nil
+           |})
         | Star l r =>
-          let (vl, hl) := hash' nextVar vs l in
-          let (vr, hr) := hash' (nextVar + length vl) vs r in
+          let (vl, hl) := hash l in
+          let (vr, hr) := hash r in
+          let nr := length vr in
           (vl ++ vr,
-            star_SHeap hl hr)
+            star_SHeap (sheap_liftVars 0 nr hl) (sheap_liftVars nr (length vl) hr))
         | Exists t b =>
-          let (v, b) := hash' (S nextVar) (nextVar :: vs) b in
+          let (v, b) := hash b in
           (t :: v, b)
         | Func f a =>
           (nil,
-           {| impures := FM.add f (map (substV vs) a :: nil) FM.empty
+           {| impures := FM.add f (a :: nil) FM.empty
             ; pures := nil
             ; other := nil
            |})
@@ -400,8 +397,6 @@ Module Make (ST' : SepTheoryX.SepTheoryXType) <: SepExprType with Module ST := S
             ; other := c :: nil
             |})
       end.
-
-    Definition hash := hash' O nil.
  
     Definition starred (T : Type) (F : T -> sexpr) (ls : list T) (base : sexpr)
       : sexpr :=
@@ -428,9 +423,9 @@ Module Make (ST' : SepTheoryX.SepTheoryXType) <: SepExprType with Module ST := S
       Star a (Star c e).
 
     Lemma starred_starred' : forall a c cs T F F' base base' ls, 
-      heq a a c cs base base' ->
-      (forall x, heq a a c cs (F x) (F' x)) ->
-      heq a a c cs (@starred T F ls base) (@starred' T F' ls base').
+      heq a c cs base base' ->
+      (forall x, heq a c cs (F x) (F' x)) ->
+      heq a c cs (@starred T F ls base) (@starred' T F' ls base').
     Proof.
       induction ls; simpl; intros.
         assumption.
@@ -442,7 +437,7 @@ Module Make (ST' : SepTheoryX.SepTheoryXType) <: SepExprType with Module ST := S
     Qed.
 
     Lemma starred'_base : forall a c cs T F base ls, 
-      heq a a c cs (Star (@starred' T F ls Emp) base) (@starred' T F ls base).
+      heq a c cs (Star (@starred' T F ls Emp) base) (@starred' T F ls base).
     Proof.
       unfold heq in *; simpl in *.
       induction ls; simpl; intros.
@@ -451,7 +446,7 @@ Module Make (ST' : SepTheoryX.SepTheoryXType) <: SepExprType with Module ST := S
     Qed.
 
     Lemma starred_base : forall a c cs T F base ls, 
-      heq a a c cs (Star (@starred T F ls Emp) base) (@starred T F ls base).
+      heq a c cs (Star (@starred T F ls Emp) base) (@starred T F ls base).
     Proof.
       unfold heq in *; simpl in *.
       induction ls; simpl; intros.
@@ -463,7 +458,7 @@ Module Make (ST' : SepTheoryX.SepTheoryXType) <: SepExprType with Module ST := S
     Qed.
 
     Lemma fold_starred : forall X a c cs (F : nat -> X -> sexpr) m b,
-      heq a a c cs (FM.fold (fun k ls a => Star (F k ls) a) m b)
+      heq a c cs (FM.fold (fun k ls a => Star (F k ls) a) m b)
       (Star (FM.fold (fun k ls a => Star (F k ls) a) m Emp) b).
     Proof.
       induction m; simpl; intros.
@@ -474,39 +469,36 @@ Module Make (ST' : SepTheoryX.SepTheoryXType) <: SepExprType with Module ST := S
     Qed.
 
     Lemma impures' : forall a c cs i b, 
-      heq a a c cs (FM.fold (fun k => starred (Func k)) i b)
+      heq a c cs (FM.fold (fun k => starred (Func k)) i b)
       (Star (FM.fold (fun k ls a => Star (starred' (Func k) ls Emp) a) i Emp) b).
     Proof.
       induction i; simpl; intros.
       autorewrite with hprop. reflexivity.
-(*
-      rewrite IHi2. rewrite <- starred_base. rewrite IHi1.
+
+      rewrite IHi2.    
+      rewrite <- (@starred_base a c cs). 
+      rewrite IHi1.
       symmetry. 
       rewrite fold_starred. repeat rewrite heq_star_assoc.
       apply heq_star_frame. reflexivity.
       apply heq_star_frame; try reflexivity.
-      rewrite starred_starred'; try reflexivity. 
+      rewrite starred_starred'; try reflexivity.
     Qed.
-*)
-    Admitted.
 
     Theorem sheapD_sheapD' : forall a c cs h, 
-      heq a a c cs (sheapD h) (sheapD' h).
+      heq a c cs (sheapD h) (sheapD' h).
     Proof.
-(*
       destruct h; unfold sheapD, sheapD'; simpl.
-      rewrite impures'. rewrite <- starred_base. 
-      rewrite <- starred_base with (ls := other0).
+      rewrite impures'. rewrite <- (@starred_base a c cs). 
+      rewrite <- (@starred_base a c cs) with (ls := other0).
       eapply heq_star_frame. reflexivity.
       eapply heq_star_frame. eapply starred_starred'; reflexivity.
       autorewrite with hprop.
       eapply starred_starred'; reflexivity.
     Qed.
-*)
-    Admitted.
 
     Lemma starred_In : forall T (F : T -> sexpr) a c cs x ls' b ls,
-      heq a a c cs (starred F (ls ++ x :: ls') b) (Star (starred F (ls ++ ls') b) (F x)).
+      heq a c cs (starred F (ls ++ x :: ls') b) (Star (starred F (ls ++ ls') b) (F x)).
     Proof.
       induction ls; intros.
         symmetry; rewrite heq_star_comm.
@@ -527,7 +519,7 @@ Module Make (ST' : SepTheoryX.SepTheoryXType) <: SepExprType with Module ST := S
       Focus 2. instantiate (1 := sexprD uvars vars (sheapD' h)). 
       match goal with
         | [ |- ?G ] => 
-          change G with (himp uvars uvars vars cs (sheapD h) (sheapD' h))
+          change G with (himp uvars vars cs (sheapD h) (sheapD' h))
       end.
       rewrite sheapD_sheapD'. reflexivity.
       
@@ -562,9 +554,9 @@ Module Make (ST' : SepTheoryX.SepTheoryXType) <: SepExprType with Module ST := S
                     pures := pures0;
                     other := other0 |}) Emp)))).
       match goal with
-        | [ |- ST.himp ?C (sexprD ?U1 ?V ?L) (sexprD ?U2 ?V ?R) ] =>
-          change (ST.himp C (sexprD U1 V L) (sexprD U2 V R)) with
-            (himp U1 U2 V C L R)
+        | [ |- ST.himp ?C (sexprD ?U ?V ?L) (sexprD ?U ?V ?R) ] =>
+          change (ST.himp C (sexprD U V L) (sexprD U V R)) with
+            (himp U V C L R)
       end.
 
       simpl. rewrite heq_star_comm. rewrite heq_star_assoc.
@@ -587,7 +579,7 @@ Module Make (ST' : SepTheoryX.SepTheoryXType) <: SepExprType with Module ST := S
     Qed.
 
     Lemma insert_at_right_star : forall a c cs i1 i2 b, 
-      heq a a c cs (FM.fold
+      heq a c cs (FM.fold
         (fun (k : nat) (ls : list (list (expr types)))
           (acc : sexpr) =>
           Star (starred' (Func k) ls Emp) acc)
@@ -619,7 +611,7 @@ Module Make (ST' : SepTheoryX.SepTheoryXType) <: SepExprType with Module ST := S
 
     Lemma sheapD_pull_impure : forall a c cs h f argss,
       FM.find f (impures h) = Some argss ->
-      heq a a c cs (sheapD h)
+      heq a c cs (sheapD h)
                    (Star (sheapD {| impures := FM.remove f (impures h)
                                   ; pures   := pures h
                                   ; other   := other h |})
@@ -657,7 +649,7 @@ Module Make (ST' : SepTheoryX.SepTheoryXType) <: SepExprType with Module ST := S
 
       rewrite insert_at_right_star.
       rewrite fold_starred.
-      symmetry. rewrite heq_star_comm. (* rewrite <- heq_star_assoc.
+      symmetry. rewrite heq_star_comm. rewrite <- (@heq_star_assoc a c cs).
       rewrite heq_star_comm. reflexivity.
 
       intros.
@@ -668,8 +660,6 @@ Module Make (ST' : SepTheoryX.SepTheoryXType) <: SepExprType with Module ST := S
       symmetry. rewrite heq_star_comm. rewrite heq_star_assoc.
       reflexivity.
     Qed.
-*)
-    Admitted.
 
     Fixpoint existsEach (ls : list tvar) {struct ls} : sexpr -> sexpr :=
       match ls with
@@ -678,43 +668,219 @@ Module Make (ST' : SepTheoryX.SepTheoryXType) <: SepExprType with Module ST := S
       end.
     
     Lemma heq_ex : forall X Y cs t P Q,
-      (forall v : tvarD types t, heq X X (existT (tvarD types) t v :: Y) cs P Q) ->
-      heq X X Y cs (Exists t P) (Exists t Q).
+      (forall v : tvarD types t, heq X (existT (tvarD types) t v :: Y) cs P Q) ->
+      heq X Y cs (Exists t P) (Exists t Q).
     Proof.
       unfold heq; simpl; intros; apply ST.heq_ex; auto.
     Qed.
 
     Lemma existsEach_heq : forall cs X v Y (P Q : sexpr),
-      (forall Z, heq X X (Z ++ Y) cs P Q) ->
-      heq X X Y cs (existsEach v P) (existsEach v Q).
+      (forall Z, map (@projT1 _ _) Z = rev v -> heq X (Z ++ Y) cs P Q) ->
+      heq X Y cs (existsEach v P) (existsEach v Q).
     Proof.
       induction v; simpl; intros.
-        apply (H nil).
-        eapply heq_ex. intros.
-        eapply IHv. intros. specialize (H (Z ++ existT (tvarD types) a v0 :: nil)).
-        rewrite app_ass in *. simpl in *. eauto.
+        specialize (H nil); simpl in *; auto.
+
+        apply heq_ex. intros. eapply IHv. intros.
+        simpl. specialize (H (Z ++ @existT _ _ _ v0 :: nil)). rewrite map_app in *. 
+        rewrite H0 in *. simpl in *.
+        rewrite app_ass in *. simpl in *. auto.
     Qed.
 
     Lemma existsEach_app : forall X cs b a Y (P : sexpr),
-      heq X X Y cs (existsEach a (existsEach b P)) (existsEach (a ++ b) P).
+      heq X Y cs (existsEach a (existsEach b P)) (existsEach (a ++ b) P).
     Proof.
       induction a; simpl.
         reflexivity.
-        intros. apply heq_ex. intros. eauto.
+        intros. apply heq_ex; intros. apply IHa.
     Qed.
 
-    Theorem hash_denote : forall cs (s : sexpr) EG G, 
-      heq EG EG G cs s 
-        (@existsEach (fst (hash s)) (sheapD (snd (hash s)))).
-    (*Proof.
-      induction s; simpl; try (unfold sheapD; reflexivity).
-        intros.
-        rewrite IHs1 at 1. rewrite IHs2 at 1. clear IHs1 IHs2.
-        destruct (hash s1); destruct (hash s2); simpl. clear. admit.
-        
-        destruct (hash s); simpl in *. intros. apply heq_ex. intros. eauto.
-    Qed.*)
+    Lemma liftSExpr_0 : forall b a, liftSExpr a 0 b = b.
+    Proof.
+      induction b; simpl; intros; auto.
+      rewrite liftExpr_0; reflexivity.
+      rewrite IHb1; rewrite IHb2; reflexivity.
+      rewrite IHb. auto.
+      f_equal. clear. induction l; simpl; auto. rewrite liftExpr_0. f_equal; auto.
+    Qed.
+
+    Lemma sexpr_lift_ext : forall EG cs G G' s G'',
+      ST.heq cs (sexprD EG (G'' ++ G) s) (sexprD EG (G'' ++ G' ++ G) (liftSExpr (length G'') (length G') s)).
+    Proof.
+      induction s; simpl; intros; 
+        repeat match goal with
+                 | [ |- _ ] => rewrite <- liftExpr_ext
+                 | [ H : forall a, ST.heq _ _ _ |- _ ] => rewrite <- H
+               end; try reflexivity.
+      eapply ST.heq_ex. intros. specialize (IHs (existT (tvarD types) t v :: G'')).
+      simpl in *. auto.
+      destruct (nth_error sfuncs f); try reflexivity.
+      clear. destruct s; simpl; clear. generalize dependent SDomain0. induction l; simpl; try reflexivity.
+      destruct SDomain0; try reflexivity.
+      rewrite <- liftExpr_ext. destruct (exprD funcs EG (G'' ++ G) a t); try reflexivity.
+      auto.
+    Qed.
+
+    Lemma star_pull_exists : forall EG cs a G s s2,
+      heq EG G cs (Star (Exists a s) s2) (Exists a (Star s (liftSExpr 0 1 s2))).
+    Proof.
+      intros. unfold heq. simpl. rewrite ST.heq_ex_star. apply ST.heq_ex. intros.
+      apply ST.heq_star_cancel.
+      generalize (sexpr_lift_ext EG cs G (existT (tvarD types) a v :: nil) s2 nil); simpl; intro. auto.
+    Qed.            
+
+    Lemma liftSExpr_combine : forall s a b c,
+      liftSExpr a b (liftSExpr a c s) = liftSExpr a (c + b) s.
+    Proof.
+      clear. induction s; intros; simpl; 
+      repeat match goal with
+               | [ H : _ |- _ ] => rewrite H
+             end; try reflexivity. 
+      rewrite liftExpr_combine. reflexivity.
+      f_equal. rewrite map_map. apply map_ext. intros; apply liftExpr_combine.
+    Qed.
+
+    Lemma star_pull_existsEach : forall EG cs v G s s2,
+      heq EG G cs (Star (existsEach v s) s2)
+      (existsEach v (Star s (liftSExpr 0 (length v) s2))).
+    Proof.
+      induction v; simpl.
+      intros; rewrite liftSExpr_0. reflexivity.
+
+      intros.
+      rewrite star_pull_exists. apply heq_ex. intros.
+      rewrite IHv.
+     
+      rewrite liftSExpr_combine. reflexivity.
+    Qed.
+
+    Lemma FM_fold_fold_right : forall T U (F : nat -> T -> U -> U) m base,
+      exists l, (forall k, In k l <-> FM.find (fst k) m = Some (snd k)) /\
+        FM.fold F m base = fold_right (fun x => F (fst x) (snd x)) base l.
+    Proof.
+      induction m; intros.
+        exists nil. simpl. intuition. congruence.
+        simpl. edestruct IHm1. intuition.
+        rewrite H1. edestruct IHm2. destruct H. erewrite H2.
+        exists (x0 ++ (n,t) :: x); split; [ | rewrite fold_right_app; reflexivity ].
+          split. intros. apply in_app_or in H3.
     Admitted.
+
+(*
+    Lemma multimap_join_ext : forall m1 m2 k,
+      FM.fold F (multimap_join m1 m2) = 
+        FM.
+        match FM.find k m1 , FM.find k m2 with
+          | None , None => None
+          | Some l , Some r => Some (l ++ r)
+          | None , r => r
+          | l , None => l
+        end.
+    Proof.
+      clear. induction m1; simpl; intros.
+      destruct (FM.find k m2); reflexivity.
+      rewrite IHm1_2. rewrite IHm1_1.
+
+case_eq (multimap_join m1_1 m2); intros; simpl.
+      destruct (FM.find k m1_2); destruct (Compare_dec.lt_eq_lt_dec k n); auto.
+        destruct s; auto.
+      P (multimap_join 
+*)
+
+
+    Lemma sheapD'_star : forall EG G cs s1 s2,
+      heq EG G cs (sheapD' (star_SHeap s1 s2)) (Star (sheapD' s1) (sheapD' s2)).
+    Proof.
+      destruct s1; destruct s2; intros; simpl; unfold sheapD', star_SHeap; simpl.
+      match goal with
+        | [ |- heq _ _ _ _ (Star (Star ?FL (Star ?PL ?OL)) (Star ?FR (Star ?PR ?OR))) ] =>
+          transitivity (Star (Star FL FR) (Star (Star PL PR) (Star OL OR)))
+      end.
+      repeat apply heq_star_frame.
+      Focus.
+      clear. unfold multimap_join. admit.
+
+      clear; induction pures0; simpl.
+        rewrite heq_star_emp_l. reflexivity.
+        rewrite heq_star_assoc. rewrite IHpures0. reflexivity.
+
+      clear; induction other0; simpl.
+        rewrite heq_star_emp_l; reflexivity.
+        rewrite heq_star_assoc. rewrite IHother0. reflexivity.
+
+      repeat (repeat rewrite heq_star_assoc; repeat (eapply heq_star_frame; [ reflexivity | ]); rewrite heq_star_comm).
+      (repeat rewrite heq_star_assoc; repeat (eapply heq_star_frame; [ reflexivity | ])). reflexivity.
+    Qed.
+
+    Lemma sheapD'_sexprD_liftVars : forall EG G cs a b s,
+      heq EG G cs (liftSExpr a b (sheapD' s)) (sheapD' (sheap_liftVars a b s)).
+    Proof.
+      destruct s; unfold sheap_liftVars, sheapD'; simpl; repeat apply heq_star_frame.
+        change Emp with (liftSExpr a b Emp) at 4; generalize Emp at 2 4.
+        induction impures0; simpl; try reflexivity; intros.
+        rewrite IHimpures0_2. rewrite fold_starred. symmetry. rewrite fold_starred. symmetry.
+        apply heq_star_frame; try reflexivity. simpl.
+        rewrite IHimpures0_1. apply heq_star_frame; try reflexivity. clear.
+        change Emp with (liftSExpr a b Emp) at 2. generalize Emp; induction t; simpl; try reflexivity.
+          intros; rewrite IHt; reflexivity.
+
+        clear; change Emp with (liftSExpr a b Emp) at 2. generalize Emp; induction pures0; simpl; try reflexivity.
+          intros; rewrite IHpures0; reflexivity.
+          
+        clear; change Emp with (liftSExpr a b Emp) at 2. generalize Emp; induction other0; try reflexivity; intros.
+          simpl; rewrite IHother0. reflexivity.
+    Qed.
+
+    Lemma liftSExpr_existsEach : forall EG cs v0 s G n v,
+      heq EG G cs (liftSExpr n v (existsEach v0 s)) 
+                  (existsEach v0 (liftSExpr (n + length v0) v s)).
+    Proof.
+      induction v0; simpl; intros.
+        intros. rewrite Plus.plus_0_r. reflexivity.
+      
+        apply heq_ex; intros. rewrite IHv0. cutrewrite (S n + length v0 = n + S (length v0)); try reflexivity; omega.
+    Qed.
+
+    Theorem hash_denote' : forall EG cs (s : sexpr) G, 
+      heq EG G cs s (@existsEach (fst (hash s)) (sheapD' (snd (hash s)))).
+    Proof.
+      Opaque star_SHeap.
+      induction s; simpl; try solve [ unfold sheapD'; simpl; intros; repeat (rewrite heq_star_emp_r || rewrite heq_star_emp_l); reflexivity ].
+        (** Exists **)
+        Focus 2.
+        unfold sheapD'; simpl; intros. case_eq (hash s); intros; simpl.
+        eapply heq_ex. intros. specialize (IHs (existT (tvarD types) t v0 :: G)). simpl in *.
+        rewrite H in IHs. simpl in *. eauto.
+
+        (** Star **)
+        Focus.
+        intros. rewrite IHs1 at 1. destruct (hash s1); destruct (hash s2); simpl in *.
+        rewrite IHs2.
+        rewrite <- (@existsEach_app EG cs) with (Y := G).
+        rewrite star_pull_existsEach. apply existsEach_heq. intros.
+        rewrite heq_star_comm.
+
+        rewrite liftSExpr_existsEach.
+        rewrite star_pull_existsEach. eapply existsEach_heq; intros.
+        rewrite sheapD'_star. simpl plus.
+        repeat rewrite sheapD'_sexprD_liftVars. rewrite heq_star_comm. reflexivity.
+    Qed.
+    
+    Theorem hash_denote : forall EG cs (s : sexpr) G, 
+      heq EG G cs s (@existsEach (fst (hash s)) (sheapD (snd (hash s)))).
+    Proof.
+      intros. specialize (@hash_denote' EG cs s G). etransitivity.
+      eassumption. apply existsEach_heq. intros. rewrite sheapD_sheapD'. reflexivity.
+    Qed.
+(*
+            Lemma fold_star_acc : forall T EG G cs (F : nat -> T -> sexpr -> sexpr) i a a',
+              heq EG G cs a a' ->
+              (forall n a b b', heq EG G cs b b' -> heq EG G cs (F n a b) (F n a b')) ->
+              heq EG G cs (FM.fold F i a) (FM.fold F i a').
+            Proof.
+              induction i; simpl; eauto.
+            Qed.
+*)
 
     (** replace "real" variables [a,b) and replace them with
      ** uvars [c,..]
@@ -856,13 +1022,13 @@ Module Make (ST' : SepTheoryX.SepTheoryXType) <: SepExprType with Module ST := S
   Lemma change_ST_himp_himp : forall (types : list type)
     (funcs : functions types) (pc st : tvar)
     (sfuncs : list (ssignature types pc st))
-    
+    EG G
     (cs : codeSpec (tvarD types pc) (tvarD types st))
     (L R : sexpr types pc st),
-    himp funcs sfuncs nil nil nil cs L R ->
+    himp funcs sfuncs EG G cs L R ->
     ST.himp cs
-      (@sexprD types pc st funcs sfuncs nil nil L)
-      (@sexprD types pc st funcs sfuncs nil nil R).
+      (@sexprD types pc st funcs sfuncs EG G L)
+      (@sexprD types pc st funcs sfuncs EG G R).
   Proof.
     unfold himp. intros. auto.
   Qed.
